imp main exercises

Imp.v
@@ -168,3 +168,506 @@ Proof.
 Qed.
 
 
+Module aevalR_first_try.
+
+Inductive aevalR : aexp -> nat -> Prop :=
+| E_ANum: forall (n: nat),
+    aevalR (ANum n) n
+| E_APlus: forall (e1 e2: aexp) (n1 n2: nat),
+    aevalR e1 n1 ->
+    aevalR e2 n2 ->
+    aevalR (APlus e1 e2) (n1 + n2)
+| E_AMinus: forall (e1 e2: aexp) (n1 n2: nat),
+    aevalR e1 n1 ->
+    aevalR e2 n2 ->
+    aevalR (AMinus e1 e2) (n1 - n2)
+| E_AMult: forall (e1 e2: aexp) (n1 n2: nat),
+    aevalR e1 n1 ->
+    aevalR e2 n2 ->
+    aevalR (AMult e1 e2) (n1 * n2).
+
+
+Notation "e '\\' n"
+         := (aevalR e n)
+            (at level 50, left associativity)
+         : type_scope.
+
+End aevalR_first_try.
+
+Reserved Notation "e '\\' n" (at level 50, left associativity).
+
+Inductive aevalR : aexp -> nat -> Prop :=
+  | E_ANum : forall (n:nat),
+      (ANum n) \\ n
+  | E_APlus : forall (e1 e2: aexp) (n1 n2 : nat),
+      (e1 \\ n1) -> (e2 \\ n2) -> (APlus e1 e2) \\ (n1 + n2)
+  | E_AMinus : forall (e1 e2: aexp) (n1 n2 : nat),
+      (e1 \\ n1) -> (e2 \\ n2) -> (AMinus e1 e2) \\ (n1 - n2)
+  | E_AMult :  forall (e1 e2: aexp) (n1 n2 : nat),
+      (e1 \\ n1) -> (e2 \\ n2) -> (AMult e1 e2) \\ (n1 * n2)
+
+  where "e '\\' n" := (aevalR e n) : type_scope.
+
+Theorem aeval_iff_aevalR : forall a n,
+  (a \\ n) <-> aeval a = n.
+Proof.
+  intros.
+  split.
+  - intros.
+    induction H; subst; reflexivity.
+  - intros. generalize dependent n.
+    induction a; simpl; intros; subst; constructor;
+      try apply IHa1; try apply IHa2; reflexivity.
+Qed.
+
+Inductive bevalR: bexp -> bool -> Prop :=
+  | E_BTrue: bevalR BTrue true
+  | E_BFalse: bevalR BFalse false
+  | E_BEq: forall (e1 e2: aexp) (n1 n2: nat),
+      (aevalR e1 n1) -> (aevalR e2 n2) ->
+      (bevalR (BEq e1 e2) (beq_nat n1 n2))
+  | E_BLe: forall (e1 e2: aexp) (n1 n2: nat),
+      (aevalR e1 n1) -> (aevalR e2 n2) ->
+      (bevalR (BLe e1 e2) (leb n1 n2))
+  | E_BNot: forall (e: bexp) (b: bool),
+      (bevalR e b) ->
+      (bevalR (BNot e) (negb b))
+  | E_BAnd: forall (e1 e2: bexp) (b1 b2: bool),
+      (bevalR e1 b1) -> (bevalR e2 b2) ->
+      (bevalR (BAnd e1 e2) (andb b1 b2)).
+
+
+
+Lemma beval_iff_bevalR : forall b bv,
+  bevalR b bv <-> beval b = bv.
+Proof.
+  intros. split.
+  - intros.
+    induction H; subst; simpl;
+      try reflexivity;
+      try (rewrite aeval_iff_aevalR in H, H0;
+           rewrite H, H0;
+           reflexivity).
+  - intros. generalize dependent bv.
+    induction b; simpl; intros; subst; constructor;
+      try (apply aeval_iff_aevalR; reflexivity);
+      try (apply IHb; reflexivity);
+      try (apply IHb1; reflexivity);
+      try (apply IHb2; reflexivity).
+Qed.
+
+
+End AExp.
+
+Module aevalR_division.
+
+Inductive aexp : Type :=
+  | ANum : nat -> aexp
+  | APlus : aexp -> aexp -> aexp
+  | AMinus : aexp -> aexp -> aexp
+  | AMult : aexp -> aexp -> aexp
+  | ADiv : aexp -> aexp -> aexp.
+
+Reserved Notation "e '\\' n"
+                  (at level 50, left associativity).
+
+Inductive aevalR : aexp -> nat -> Prop :=
+  | E_ANum : forall (n:nat),
+      (ANum n) \\ n
+  | E_APlus : forall (a1 a2: aexp) (n1 n2 : nat),
+      (a1 \\ n1) -> (a2 \\ n2) -> (APlus a1 a2) \\ (n1 + n2)
+  | E_AMinus : forall (a1 a2: aexp) (n1 n2 : nat),
+      (a1 \\ n1) -> (a2 \\ n2) -> (AMinus a1 a2) \\ (n1 - n2)
+  | E_AMult :  forall (a1 a2: aexp) (n1 n2 : nat),
+      (a1 \\ n1) -> (a2 \\ n2) -> (AMult a1 a2) \\ (n1 * n2)
+  | E_ADiv :  forall (a1 a2: aexp) (n1 n2 n3: nat),
+      (a1 \\ n1) -> (a2 \\ n2) -> (n2 > 0) ->
+      (mult n2 n3 = n1) -> (ADiv a1 a2) \\ n3
+
+where "a '\\' n" := (aevalR a n) : type_scope.
+
+End aevalR_division.
+
+
+Module aevalR_extended.
+
+Reserved Notation "e '\\' n" (at level 50, left associativity).
+
+Inductive aexp : Type :=
+  | AAny  : aexp                   (* <--- NEW *)
+  | ANum : nat -> aexp
+  | APlus : aexp -> aexp -> aexp
+  | AMinus : aexp -> aexp -> aexp
+  | AMult : aexp -> aexp -> aexp.
+
+
+Inductive aevalR : aexp -> nat -> Prop :=
+  | E_Any : forall (n:nat),
+      AAny \\ n                 (* <--- new *)
+  | E_ANum : forall (n:nat),
+      (ANum n) \\ n
+  | E_APlus : forall (a1 a2: aexp) (n1 n2 : nat),
+      (a1 \\ n1) -> (a2 \\ n2) -> (APlus a1 a2) \\ (n1 + n2)
+  | E_AMinus : forall (a1 a2: aexp) (n1 n2 : nat),
+      (a1 \\ n1) -> (a2 \\ n2) -> (AMinus a1 a2) \\ (n1 - n2)
+  | E_AMult :  forall (a1 a2: aexp) (n1 n2 : nat),
+      (a1 \\ n1) -> (a2 \\ n2) -> (AMult a1 a2) \\ (n1 * n2)
+
+where "a '\\' n" := (aevalR a n) : type_scope.
+
+End aevalR_extended.
+
+Definition state := total_map nat.
+
+Definition empty_state : state :=
+  t_empty 0.
+
+Inductive aexp : Type :=
+  | ANum : nat -> aexp
+  | AId : id -> aexp
+  | APlus : aexp -> aexp -> aexp
+  | AMinus : aexp -> aexp -> aexp
+  | AMult : aexp -> aexp -> aexp.
+
+Definition W : id := Id "W".
+Definition X : id := Id "X".
+Definition Y : id := Id "Y".
+Definition Z : id := Id "Z".
+
+Inductive bexp : Type :=
+  | BTrue : bexp
+  | BFalse : bexp
+  | BEq : aexp -> aexp -> bexp
+  | BLe : aexp -> aexp -> bexp
+  | BNot : bexp -> bexp
+  | BAnd : bexp -> bexp -> bexp.
+
+Fixpoint aeval (st : state) (a : aexp) : nat :=
+  match a with
+  | ANum n => n
+  | AId x => st x     (* <----- NEW *)
+  | APlus a1 a2 => (aeval st a1) + (aeval st a2)
+  | AMinus a1 a2  => (aeval st a1) - (aeval st a2)
+  | AMult a1 a2 => (aeval st a1) * (aeval st a2)
+  end.
+Fixpoint beval (st : state) (b : bexp) : bool :=
+  match b with
+  | BTrue       => true
+  | BFalse      => false
+  | BEq a1 a2   => beq_nat (aeval st a1) (aeval st a2)
+  | BLe a1 a2   => leb (aeval st a1) (aeval st a2)
+  | BNot b1     => negb (beval st b1)
+  | BAnd b1 b2  => andb (beval st b1) (beval st b2)
+  end.
+
+Example aexp1 :
+  aeval (t_update empty_state X 5)
+        (APlus (ANum 3) (AMult (AId X) (ANum 2)))
+  = 13.
+Proof. reflexivity. Qed.
+
+Example bexp1 :
+  beval (t_update empty_state X 5)
+        (BAnd BTrue (BNot (BLe (AId X) (ANum 4))))
+  = true.
+Proof. reflexivity. Qed.
+
+Inductive com : Type :=
+  | CSkip : com
+  | CAss : id -> aexp -> com
+  | CSeq : com -> com -> com
+  | CIf : bexp -> com -> com -> com
+  | CWhile : bexp -> com -> com.
+
+Notation "'SKIP'" :=
+  CSkip.
+Notation "x '::=' a" :=
+  (CAss x a) (at level 60).
+Notation "c1 ;; c2" :=
+  (CSeq c1 c2) (at level 80, right associativity).
+Notation "'WHILE' b 'DO' c 'END'" :=
+  (CWhile b c) (at level 80, right associativity).
+Notation "'IFB' b1 'THEN' c2 'ELSE' c3 'FI'" :=
+  (CIf b1 c2 c3) (at level 80, right associativity).
+
+Definition fact_in_coq : com :=
+  Z ::= AId X;;
+  Y ::= ANum 1;;
+  WHILE BNot (BEq (AId Z) (ANum 0)) DO
+    Y ::= AMult (AId Y) (AId Z);;
+    Z ::= AMinus (AId Z) (ANum 1)
+  END.
+
+Definition plus2 : com :=
+  X ::= (APlus (AId X) (ANum 2)).
+
+Definition XtimesYinZ : com :=
+  Z ::= (AMult (AId X) (AId Y)).
+
+Definition subtract_slowly_body : com :=
+  Z ::= AMinus (AId Z) (ANum 1) ;;
+  X ::= AMinus (AId X) (ANum 1).
+
+Definition subtract_slowly : com :=
+  WHILE BNot (BEq (AId X) (ANum 0)) DO
+    subtract_slowly_body
+  END.
+
+Definition subtract_3_from_5_slowly : com :=
+  X ::= ANum 3 ;;
+  Z ::= ANum 5 ;;
+  subtract_slowly.
+
+Definition loop : com :=
+  WHILE BTrue DO
+    SKIP
+  END.
+
+Reserved Notation "c1 '/' st '\\' st'"
+                  (at level 40, st at level 39).
+
+Inductive ceval : com -> state -> state -> Prop :=
+| E_Skip: forall st,
+    SKIP / st \\ st
+| E_Ass: forall st ae x n,
+    aeval st ae = n ->
+    (x ::= ae) / st \\ (t_update st x n)
+| E_Seq: forall c1 c2 st st' st'',
+    c1 / st \\ st' ->
+    c2 / st' \\ st'' ->
+    (c1 ;; c2) / st \\ st''
+| E_IfTrue: forall b1 c1 c2 st st',
+    beval st b1 = true ->
+    c1 / st \\ st' ->
+    (IFB b1 THEN c1 ELSE c2 FI) / st \\ st'
+| E_IfFalse: forall b1 c1 c2 st st',
+    beval st b1 = false ->
+    c2 / st \\ st' ->
+    (IFB b1 THEN c1 ELSE c2 FI) / st \\ st'
+| E_WhileEnd: forall b1 c1 st,
+    beval st b1 = false ->
+    (WHILE b1 DO c1 END) / st \\ st
+| E_WhileLoop: forall b1 c1 st st' st'',
+    beval st b1 = true ->
+    c1 / st \\ st' ->
+    (WHILE b1 DO c1 END) / st' \\ st'' ->
+    (WHILE b1 DO c1 END) / st \\ st''
+
+    where "c1 '/' st '\\' st'" := (ceval c1 st st').
+
+
+Example ceval_example1:
+    (X ::= ANum 2;;
+     IFB BLe (AId X) (ANum 1)
+       THEN Y ::= ANum 3
+       ELSE Z ::= ANum 4
+     FI)
+   / empty_state
+   \\ (t_update (t_update empty_state X 2) Z 4).
+Proof.
+  apply E_Seq with (t_update empty_state X 2).
+  - apply E_Ass. reflexivity.
+  - apply E_IfFalse.
+    + reflexivity.
+    + apply E_Ass. reflexivity.
+Qed.
+
+Example ceval_example2:
+    (X ::= ANum 0;; Y ::= ANum 1;; Z ::= ANum 2) / empty_state \\
+    (t_update (t_update (t_update empty_state X 0) Y 1) Z 2).
+Proof.
+  apply E_Seq with (t_update empty_state X 0).
+  - apply E_Ass. reflexivity.
+  - apply E_Seq with (t_update (t_update empty_state X 0) Y 1).
+    + apply E_Ass. reflexivity.
+    + apply E_Ass. reflexivity.
+Qed.
+
+Definition pup_to_n : com :=
+  Y ::= (ANum 0);;
+  WHILE BLe (ANum 1) (AId X)
+     DO Y ::= (APlus (AId Y) (AId X));;
+        X ::= (AMinus (AId X) (ANum 1))
+    END.
+
+
+Theorem pup_to_2_ceval :
+  pup_to_n / (t_update empty_state X 2) \\
+    t_update (t_update (t_update (t_update (t_update (t_update empty_state X 2) Y 0) Y 2) X 1) Y 3) X 0.
+Proof.
+  apply E_Seq with (t_update (t_update empty_state X 2) Y 0).
+  - apply E_Ass. reflexivity.
+  - apply E_WhileLoop with (t_update (t_update (t_update (t_update empty_state X 2) Y 0) Y 2) X 1).
+    + reflexivity.
+    + apply E_Seq with (t_update (t_update (t_update empty_state X 2) Y 0) Y 2).
+      * apply E_Ass. reflexivity.
+      * apply E_Ass. reflexivity.
+    + apply E_WhileLoop with (t_update (t_update (t_update (t_update (t_update (t_update empty_state X 2) Y 0) Y 2) X 1) Y 3) X 0).
+      * reflexivity.
+      * apply E_Seq with  (t_update (t_update (t_update (t_update (t_update empty_state X 2) Y 0) Y 2) X 1) Y 3).
+        { apply E_Ass. reflexivity. }
+        { apply E_Ass. reflexivity. }
+      * apply E_WhileEnd. reflexivity.
+Qed.
+
+Theorem ceval_deterministic: forall c st st1 st2,
+     c / st \\ st1  ->
+     c / st \\ st2 ->
+     st1 = st2.
+Proof.
+  intros.
+  generalize dependent st2.
+  induction H; intros st2 H'; inversion H'; subst.
+  - reflexivity.
+  - reflexivity.
+  - assert (st' = st'0).
+    { apply IHceval1. assumption. }
+    subst st'0.
+    apply IHceval2.
+    assumption.
+  - apply IHceval.
+    assumption.
+  - rewrite H in H6. inversion H6.
+  - rewrite H in H6. inversion H6.
+  - apply IHceval.
+    assumption.
+  - reflexivity.
+  - rewrite H in H2. inversion H2.
+  - rewrite H in H6. inversion H6.
+  - assert (st' = st'0).
+    { apply IHceval1. assumption. }
+    subst st'0.
+    apply IHceval2.
+    assumption.
+Qed.
+
+Theorem plus2_spec : forall st n st',
+  st X = n ->
+  plus2 / st \\ st' ->
+  st' X = n + 2.
+Proof.
+  intros st n st' HX Heval.
+  inversion Heval.
+  subst.
+  simpl.
+  apply t_update_eq.
+Qed.
+
+Theorem XtimesYinZ_spec : forall st x y st',
+  st X = x ->
+  st Y = y ->
+  XtimesYinZ / st \\ st' ->
+  st' Z = x * y.
+Proof.
+  intros.
+  inversion H1.
+  subst.
+  simpl.
+  apply t_update_eq.
+Qed.
+
+Theorem loop_never_stops : forall st st',
+  ~(loop / st \\ st').
+Proof.
+  intros st st' contra. unfold loop in contra.
+  remember (WHILE BTrue DO SKIP END) as loopdef
+           eqn:Heqloopdef.
+  induction contra; inversion Heqloopdef.
+  - rewrite H1 in H. inversion H.
+  - apply IHcontra2. rewrite H1, H2. reflexivity.
+Qed.
+
+Fixpoint no_whiles (c : com) : bool :=
+  match c with
+  | SKIP =>
+      true
+  | _ ::= _ =>
+      true
+  | c1 ;; c2 =>
+      andb (no_whiles c1) (no_whiles c2)
+  | IFB _ THEN ct ELSE cf FI =>
+      andb (no_whiles ct) (no_whiles cf)
+  | WHILE _ DO _ END  =>
+      false
+  end.
+
+Inductive no_whilesR: com -> Prop :=
+| nw_skip: no_whilesR SKIP
+| nw_ass: forall x ex,
+    no_whilesR (x ::= ex)
+| nw_seq: forall c1 c2,
+    no_whilesR c1 ->
+    no_whilesR c2 ->
+    no_whilesR (c1 ;; c2)
+| nw_ifb: forall b c1 c2,
+    no_whilesR c1 ->
+    no_whilesR c2 ->
+    no_whilesR (IFB b THEN c1 ELSE c2 FI).
+
+Theorem no_whiles_eqv:
+   forall c, no_whiles c = true <-> no_whilesR c.
+Proof.
+  intros. split.
+  - intros.
+    induction c.
+    + apply nw_skip.
+    + apply nw_ass.
+    + simpl in H.
+      apply andb_true_iff in H.
+      destruct H.
+      apply nw_seq.
+      * apply IHc1. apply H.
+      * apply IHc2. apply H0.
+    + simpl in H.
+      apply andb_true_iff in H.
+      destruct H.
+      apply nw_ifb.
+      * apply IHc1. apply H.
+      * apply IHc2. apply H0.
+    + simpl in H. inversion H.
+  - intros.
+    induction c; simpl.
+    + reflexivity.
+    + reflexivity.
+    + inversion H. 
+      apply andb_true_iff.
+      split.
+      * apply IHc1. apply H2.
+      * apply IHc2. apply H3.
+    + inversion H.
+      apply andb_true_iff.
+      split.
+      * apply IHc1. apply H2.
+      * apply IHc2. apply H4.
+    + inversion H.
+Qed.
+
+Theorem no_whiles_terminating: forall c st,
+    no_whilesR c ->
+    exists st', c / st \\ st'.
+Proof.
+  intros.
+  generalize dependent st.
+  induction H; intros.
+  - exists st.
+    apply E_Skip.
+  - exists (t_update st x (aeval st ex)).
+    apply E_Ass. reflexivity.
+  - destruct (IHno_whilesR1 st).
+    destruct (IHno_whilesR2 x).
+    exists x0.
+    apply (E_Seq c1 c2 st x x0).
+    + apply H1.
+    + apply H2.
+  - destruct (beval st b) eqn:bval.
+    + destruct (IHno_whilesR1 st).
+      exists x.
+      apply E_IfTrue.
+      apply bval.
+      apply H1.
+    + destruct (IHno_whilesR2 st).
+      exists x.
+      apply E_IfFalse.
+      apply bval.
+      apply H1.
+Qed.
